Simplify simplereplicaset by removing the usage of chan

kubernetes_model/simplereplicaset/replica_set.go
@@ -5,67 +5,22 @@ import (
 	"fmt"
 	"kubernetes_model/simpleapiserver"
 	"sort"
-	"sync"
 
 	apps "k8s.io/api/apps/v1"
 	v1 "k8s.io/api/core/v1"
 	apierrors "k8s.io/apimachinery/pkg/api/errors"
 	metav1 "k8s.io/apimachinery/pkg/apis/meta/v1"
 	"k8s.io/apimachinery/pkg/labels"
-	"k8s.io/apimachinery/pkg/runtime/schema"
 	"k8s.io/apimachinery/pkg/types"
-	utilruntime "k8s.io/apimachinery/pkg/util/runtime"
 	"k8s.io/client-go/tools/cache"
 	"k8s.io/klog/v2"
 	"k8s.io/kubernetes/pkg/controller"
 )
 
-// ReplicaSetController is responsible for synchronizing ReplicaSet objects stored
-// in the system with actual running pods.
-type ReplicaSetController struct {
-	// GroupVersionKind indicates the controller type.
-	// Different instances of this struct may handle different GVKs.
-	// For example, this struct can be used (with adapters) to handle ReplicationController.
-	schema.GroupVersionKind
-
-	// A ReplicaSet is temporarily suspended after creating/deleting these many replicas.
-	// It resumes normal action after observing the watch events for them.
-	burstReplicas int
-}
-
-func validateControllerRef(controllerRef *metav1.OwnerReference) error {
-	if controllerRef == nil {
-		return fmt.Errorf("controllerRef is nil")
-	}
-	if len(controllerRef.APIVersion) == 0 {
-		return fmt.Errorf("controllerRef has empty APIVersion")
-	}
-	if len(controllerRef.Kind) == 0 {
-		return fmt.Errorf("controllerRef has empty Kind")
-	}
-	if controllerRef.Controller == nil || !*controllerRef.Controller {
-		return fmt.Errorf("controllerRef.Controller is not set to true")
-	}
-	if controllerRef.BlockOwnerDeletion == nil || !*controllerRef.BlockOwnerDeletion {
-		return fmt.Errorf("controllerRef.BlockOwnerDeletion is not set")
-	}
-	return nil
-}
-
-func CreatePods(ctx context.Context, namespace string, template *v1.PodTemplateSpec, controllerObject *apps.ReplicaSet, controllerRef *metav1.OwnerReference) error {
-	return CreatePodsWithGenerateName(ctx, namespace, template, controllerObject, controllerRef, "")
-}
-
-func CreatePodsWithGenerateName(ctx context.Context, namespace string, template *v1.PodTemplateSpec, controllerObject *apps.ReplicaSet, controllerRef *metav1.OwnerReference, generateName string) error {
-	if err := validateControllerRef(controllerRef); err != nil {
-		return err
-	}
+func CreatePod(ctx context.Context, namespace string, template *v1.PodTemplateSpec, controllerObject *apps.ReplicaSet, controllerRef *metav1.OwnerReference) error {
 	pod, err := controller.GetPodFromTemplate(template, controllerObject, controllerRef)
 	if err != nil {
 		return err
-	}
-	if len(generateName) > 0 {
-		pod.ObjectMeta.GenerateName = generateName
 	}
 	if len(labels.Set(pod.Labels)) == 0 {
 		return fmt.Errorf("unable to create pods, no labels")
@@ -87,7 +42,6 @@ func FilterPodsByOwner(owner *metav1.ObjectMeta) ([]*v1.Pod, error) {
 		for _, obj := range pods {
 			pod, ok := obj.(*v1.Pod)
 			if !ok {
-				utilruntime.HandleError(fmt.Errorf("unexpected object type in pod indexer: %v", obj))
 				continue
 			}
 			result = append(result, pod)
@@ -96,16 +50,14 @@ func FilterPodsByOwner(owner *metav1.ObjectMeta) ([]*v1.Pod, error) {
 	return result, nil
 }
 
-func (rsc *ReplicaSetController) getReplicaSetsWithSameController(logger klog.Logger, rs *apps.ReplicaSet) []*apps.ReplicaSet {
+func getReplicaSetsWithSameController(logger klog.Logger, rs *apps.ReplicaSet) []*apps.ReplicaSet {
 	controllerRef := metav1.GetControllerOf(rs)
 	if controllerRef == nil {
-		utilruntime.HandleError(fmt.Errorf("ReplicaSet has no controller: %v", rs))
 		return nil
 	}
 
 	objects, err := simpleapiserver.ByIndex("ReplicaSet", simpleapiserver.ControllerUIDIndex, string(controllerRef.UID))
 	if err != nil {
-		utilruntime.HandleError(err)
 		return nil
 	}
 	relatedRSs := make([]*apps.ReplicaSet, 0, len(objects))
@@ -119,80 +71,31 @@ func (rsc *ReplicaSetController) getReplicaSetsWithSameController(logger klog.Lo
 // manageReplicas checks and updates replicas for the given ReplicaSet.
 // Does NOT modify <activePods>.
 // It will requeue the replica set in case of an error while creating/deleting pods.
-func (rsc *ReplicaSetController) manageReplicas(ctx context.Context, activePods []*v1.Pod, rs *apps.ReplicaSet) error {
+func manageReplicas(ctx context.Context, activePods []*v1.Pod, rs *apps.ReplicaSet) error {
 	diff := len(activePods) - int(*(rs.Spec.Replicas))
 	_, err := controller.KeyFunc(rs)
 	if err != nil {
-		utilruntime.HandleError(fmt.Errorf("couldn't get key for %v %#v: %v", rsc.Kind, rs, err))
 		return nil
 	}
 	logger := klog.FromContext(ctx)
 	if diff < 0 {
 		diff *= -1
-		if diff > rsc.burstReplicas {
-			diff = rsc.burstReplicas
-		}
-		// TODO: Track UIDs of creates just like deletes. The problem currently
-		// is we'd need to wait on the result of a create to record the pod's
-		// UID, which would require locking *across* the create, which will turn
-		// into a performance bottleneck. We should generate a UID for the pod
-		// beforehand and store it via ExpectCreations.
-		logger.V(2).Info("Too few replicas", "replicaSet", klog.KObj(rs), "need", *(rs.Spec.Replicas), "creating", diff)
-		// Batch the pod creates. Batch sizes start at SlowStartInitialBatchSize
-		// and double with each successful iteration in a kind of "slow start".
-		// This handles attempts to start large numbers of pods that would
-		// likely all fail with the same error. For example a project with a
-		// low quota that attempts to create a large number of pods will be
-		// prevented from spamming the API service with the pod create requests
-		// after one of its pods fails.  Conveniently, this also prevents the
-		// event spam that those failures would generate.
-		_, err := slowStartBatch(diff, controller.SlowStartInitialBatchSize, func() error {
-			err := CreatePods(ctx, rs.Namespace, &rs.Spec.Template, rs, metav1.NewControllerRef(rs, rsc.GroupVersionKind))
-			if err != nil {
-				if apierrors.HasStatusCause(err, v1.NamespaceTerminatingCause) {
-					// if the namespace is being terminated, we don't have to do
-					// anything because any creation will fail
-					return nil
-				}
-			}
-			return err
-		})
-
-		return err
-	} else if diff > 0 {
-		if diff > rsc.burstReplicas {
-			diff = rsc.burstReplicas
-		}
-		logger.V(2).Info("Too many replicas", "replicaSet", klog.KObj(rs), "need", *(rs.Spec.Replicas), "deleting", diff)
-
-		relatedPods, err := rsc.getIndirectlyRelatedPods(logger, rs)
-		utilruntime.HandleError(err)
-
-		// Choose which Pods to delete, preferring those in earlier phases of startup.
-		podsToDelete := getPodsToDelete(activePods, relatedPods, diff)
-
-		errCh := make(chan error, diff)
-		var wg sync.WaitGroup
-		wg.Add(diff)
-		for _, pod := range podsToDelete {
-			go func(targetPod *v1.Pod) {
-				defer wg.Done()
-				if err := simpleapiserver.PodDelete(rs.Namespace, targetPod.Name); err != nil {
-					if !apierrors.IsNotFound(err) {
-						errCh <- err
-					}
-				}
-			}(pod)
-		}
-		wg.Wait()
-
-		select {
-		case err := <-errCh:
-			// all errors have been reported before and they're likely to be the same, so we'll only return the first one we hit.
+		for i := 0; i < diff; i++ {
+			err := CreatePod(ctx, rs.Namespace, &rs.Spec.Template, rs, metav1.NewControllerRef(rs, apps.SchemeGroupVersion.WithKind("ReplicaSet")))
 			if err != nil {
 				return err
 			}
-		default:
+		}
+	} else if diff > 0 {
+		relatedPods, _ := getIndirectlyRelatedPods(logger, rs)
+		// Choose which Pods to delete, preferring those in earlier phases of startup.
+		podsToDelete := getPodsToDelete(activePods, relatedPods, diff)
+		for _, pod := range podsToDelete {
+			if err := simpleapiserver.PodDelete(rs.Namespace, pod.Name); err != nil {
+				if !apierrors.IsNotFound(err) {
+					return err
+				}
+			}
 		}
 	}
 
@@ -202,7 +105,7 @@ func (rsc *ReplicaSetController) manageReplicas(ctx context.Context, activePods 
 // syncReplicaSet will sync the ReplicaSet with the given key if it has had its expectations fulfilled,
 // meaning it did not expect to see any more of its pods created or deleted. This function is not meant to be
 // invoked concurrently with the same key.
-func (rsc *ReplicaSetController) syncReplicaSet(ctx context.Context, key string) error {
+func syncReplicaSet(ctx context.Context, key string) error {
 	logger := klog.FromContext(ctx)
 
 	namespace, name, err := cache.SplitMetaNamespaceKey(key)
@@ -229,64 +132,18 @@ func (rsc *ReplicaSetController) syncReplicaSet(ctx context.Context, key string)
 
 	var manageReplicasErr error
 	if rs.DeletionTimestamp == nil {
-		manageReplicasErr = rsc.manageReplicas(ctx, allActivePods, rs)
+		manageReplicasErr = manageReplicas(ctx, allActivePods, rs)
 	}
 
 	return manageReplicasErr
 }
 
-// goose doesn't support Go's built-in min with final type int, so we define our own int
-func min(a, b int) int {
-	if a <= b {
-		return a
-	} else {
-		return b
-	}
-}
-
-// slowStartBatch tries to call the provided function a total of 'count' times,
-// starting slow to check for errors, then speeding up if calls succeed.
-//
-// It groups the calls into batches, starting with a group of initialBatchSize.
-// Within each batch, it may call the function multiple times concurrently.
-//
-// If a whole batch succeeds, the next batch may get exponentially larger.
-// If there are any failures in a batch, all remaining batches are skipped
-// after waiting for the current batch to complete.
-//
-// It returns the number of successful calls to the function.
-func slowStartBatch(count int, initialBatchSize int, fn func() error) (int, error) {
-	remaining := count
-	successes := 0
-	for batchSize := min(remaining, initialBatchSize); batchSize > 0; batchSize = min(2*batchSize, remaining) {
-		errCh := make(chan error, batchSize)
-		var wg sync.WaitGroup
-		wg.Add(batchSize)
-		for i := 0; i < batchSize; i++ {
-			go func() {
-				defer wg.Done()
-				if err := fn(); err != nil {
-					errCh <- err
-				}
-			}()
-		}
-		wg.Wait()
-		curSuccesses := batchSize - len(errCh)
-		successes += curSuccesses
-		if len(errCh) > 0 {
-			return successes, <-errCh
-		}
-		remaining -= batchSize
-	}
-	return successes, nil
-}
-
 // getIndirectlyRelatedPods returns all pods that are owned by any ReplicaSet
 // that is owned by the given ReplicaSet's owner.
-func (rsc *ReplicaSetController) getIndirectlyRelatedPods(logger klog.Logger, rs *apps.ReplicaSet) ([]*v1.Pod, error) {
+func getIndirectlyRelatedPods(logger klog.Logger, rs *apps.ReplicaSet) ([]*v1.Pod, error) {
 	var relatedPods []*v1.Pod
 	seen := make(map[types.UID]*apps.ReplicaSet)
-	for _, relatedRS := range rsc.getReplicaSetsWithSameController(logger, rs) {
+	for _, relatedRS := range getReplicaSetsWithSameController(logger, rs) {
 		selector, err := metav1.LabelSelectorAsSelector(relatedRS.Spec.Selector)
 		if err != nil {
 			// This object has an invalid selector, it does not match any pods
@@ -297,15 +154,13 @@ func (rsc *ReplicaSetController) getIndirectlyRelatedPods(logger klog.Logger, rs
 			return nil, err
 		}
 		for _, pod := range pods {
-			if otherRS, found := seen[pod.UID]; found {
-				logger.V(5).Info("Pod is owned by both", "pod", klog.KObj(pod), "kind", rsc.Kind, "replicaSets", klog.KObjSlice([]klog.KMetadata{otherRS, relatedRS}))
+			if _, found := seen[pod.UID]; found {
 				continue
 			}
 			seen[pod.UID] = relatedRS
 			relatedPods = append(relatedPods, pod)
 		}
 	}
-	logger.V(4).Info("Found related pods", "kind", rsc.Kind, "replicaSet", klog.KObj(rs), "pods", klog.KObjSlice(relatedPods))
 	return relatedPods, nil
 }
 
