src/verification/kubernetes_model/simplereplicaset_init.v
@@ -5,11 +5,7 @@ From verification.k8s_io.api.core Require Export v1_init.
 From verification.k8s_io.apimachinery.pkg.api Require Export errors_init.
 From verification.k8s_io.apimachinery.pkg.apis.meta Require Export v1_init.
 From verification.k8s_io.apimachinery.pkg Require Export labels_init.
-From verification.k8s_io.apimachinery.pkg.runtime Require Export schema_init.
 From verification.k8s_io.apimachinery.pkg.types Require Export types_init.
-From verification.k8s_io.apimachinery.pkg.util Require Export runtime_init.
-From verification.k8s_io.client_go.listers.apps Require Export v1_init.
-From verification.k8s_io.client_go.listers.core Require Export v1_init.
 From verification.k8s_io.client_go.tools Require Export cache_init.
 From verification.k8s_io.klog Require Export klog_init.
 From verification.k8s_io.kubernetes.pkg Require Export controller_init.
